proof/Russell/GenerationRange.v
@@ -11,7 +11,6 @@ Require Import CCPD.Coercion.
 Require Import CCPD.GenerationNotKind.
 Require Import CCPD.GenerationCoerce.
 Require Import CCPD.Generation.
-Require Import CCPD.Axioms.
 
 Implicit Types i k m n p : nat.
 Implicit Type s : sort.
@@ -28,7 +27,6 @@ Proof.
   generalize H ; clear H.
   elim (le_gt_dec k n0) ;  simpl ; intros ; try discriminate.
   apply IHt2 with (S k) ; auto.
-  apply IHt2 with (S k) ; auto.
 Qed.
 
 Lemma type_range_subst : forall t u n s, type_range (subst_rec t u n) = Srt s ->
@@ -43,7 +41,6 @@ Proof.
   unfold lift in H0.
   left ; exact (type_range_lift _ _ _ H0).
   
-  apply IHu2 with (S n) ; auto.
   apply IHu2 with (S n) ; auto.
 Qed.
 
@@ -86,227 +83,6 @@ Lemma no_sort_type_range : forall A, no_sort A -> forall s, type_range A <> Srt 
 Proof.
   induction A ; simpl ; intros ; intuition ; try discriminate ; auto.
   apply H1 with s ; auto.
-  apply H3 with s ; auto.
-Qed.
-
-Lemma is_low_type_range : forall A, forall e T, e |- A : T -> is_low_full A -> 
-  (forall s, type_range A <> Srt s) \/ 
-  (exists s, type_range A = Srt s /\ is_prop s).
-Proof.
-  induction A ;  simpl ; intros ; intuition ; try discriminate.
-
-  right.
-  exists s ; intuition.
-  
-  destruct (generation_prod H).
-  rewrite H1 in H.
-  destruct (generation_prod2 H).
-  apply IHA2 with (A1 :: e) (Srt x) ; auto.
-  
-  destruct (generation_sum H).
-  rewrite H1 in H.
-  destruct (generation_sum2 H).
-  destruct H3.
-  destruct H4.
-  destruct H4.
-  apply IHA2 with (A1 :: e) (Srt x1) ; auto.
-
-  left.
-  intros.
-  pose (no_sort_type_range _ H2 H0).
-  contradiction.
-
-  destruct (generation_sum H).
-  rewrite H0 in H.
-  destruct (generation_sum2 H).
-  destruct H3.
-  destruct H4.
-  destruct H4.
-  apply IHA2 with (A1 :: e) (Srt x1) ; auto.
-Qed.
-
-Definition is_low_sort t : Prop := t = Srt prop \/ t = Srt set.
-
-Lemma conv_is_low_range : forall A s, conv (Srt s) A -> 
-  is_low_sort (type_range A) -> A = Srt s.
-Proof.
-  induction A ; simpl ; intros ; 
-  try unfold is_low_sort in H0 ; intuition ; try discriminate ; auto with coc core datatypes.
-  
-  rewrite (conv_sort _ _ H).
-  auto.
-
-  rewrite (conv_sort _ _ H).
-  auto.
-
-  elim conv_sort_prod with s A1 A2 ; auto with coc core.
-  elim conv_sort_prod with s A1 A2 ; auto with coc core.
-
-  elim conv_sort_sum with s A1 A2 ; auto with coc core.
-  elim conv_sort_sum with s A1 A2 ; auto with coc core.
-Qed.
-
-Lemma conv_is_low_dom : forall A s, conv (Srt s) A -> 
-  is_low_sort (type_dom A) -> A = Srt s.
-Proof.
-  induction A ; simpl ; intros ; 
-  try unfold is_low_sort in H0 ; intuition ; try discriminate ; auto with coc core datatypes.
-  
-  rewrite (conv_sort _ _ H).
-  auto.
-
-  rewrite (conv_sort _ _ H).
-  auto.
-
-  elim conv_sort_prod with s A1 A2 ; auto with coc core.
-  elim conv_sort_prod with s A1 A2 ; auto with coc core.
-
-  elim conv_sort_sum with s A1 A2 ; auto with coc core.
-  elim conv_sort_sum with s A1 A2 ; auto with coc core.
-Qed.
- 
-Lemma conv_is_low_range_full : forall A B, conv A B ->
-  is_low_sort (type_range A) -> 
-  is_low_sort (type_range B) -> type_range A = type_range B.
-Proof.
-  induction A ; simpl ; intros ; 
-  try unfold is_low_sort in H0 ;   
-  intuition ; try discriminate ; auto with coc core datatypes.
-  
-  rewrite (conv_is_low_range H H1).
-  simpl ; auto.
-
-  rewrite (conv_is_low_range H H1).
-  simpl ; auto.
-  
-  induction B ; simpl ; intros ; 
-  try unfold is_low_sort in H1 ;   
-  intuition ; try discriminate ; auto with coc core datatypes.
-
-  elim conv_sort_prod with s A1 A2 ; auto with coc core.
-  elim conv_sort_prod with s A1 A2 ; auto with coc core.
-
-  simpl in H0.
-  apply (IHA2 B2 (inv_conv_prod_r _ _ _ _ H)).
-  unfold is_low_sort ; rewrite H2 ; auto.
-  unfold is_low_sort ; rewrite H0 ; auto.
-
-  simpl in H0.
-  apply (IHA2 B2 (inv_conv_prod_r _ _ _ _ H)).
-  unfold is_low_sort ; rewrite H2 ; auto.
-  unfold is_low_sort ; rewrite H0 ; auto.
-
-  elim conv_prod_sum with A1 A2 B1 B2 ; auto with coc.
-  elim conv_prod_sum with A1 A2 B1 B2 ; auto with coc.
-
-  induction B ; simpl ; intros ; 
-  try unfold is_low_sort in H1 ;   
-  intuition ; try discriminate ; auto with coc core datatypes.
-
-  elim conv_sort_prod with s A1 A2 ; auto with coc core.
-  elim conv_sort_prod with s A1 A2 ; auto with coc core.
-
-  simpl in H0.
-  apply (IHA2 B2 (inv_conv_prod_r _ _ _ _ H)).
-  unfold is_low_sort ; rewrite H2 ; auto.
-  unfold is_low_sort ; rewrite H0 ; auto.
-
-  simpl in H0.
-  apply (IHA2 B2 (inv_conv_prod_r _ _ _ _ H)).
-  unfold is_low_sort ; rewrite H2 ; auto.
-  unfold is_low_sort ; rewrite H0 ; auto.
-
-  elim conv_prod_sum with A1 A2 B1 B2 ; auto with coc.
-  elim conv_prod_sum with A1 A2 B1 B2 ; auto with coc.
-
-  induction B ; simpl ; intros ; 
-  try unfold is_low_sort in H1 ;   
-  intuition ; try discriminate ; auto with coc core datatypes.
-
-  elim conv_sort_sum with s A1 A2 ; auto with coc core.
-  elim conv_sort_sum with s A1 A2 ; auto with coc core.
-
-  elim conv_prod_sum with B1 B2 A1 A2; auto with coc core.
-  elim conv_prod_sum with B1 B2 A1 A2; auto with coc core.
-
-  simpl in H0.
-  apply (IHA2 B2 (inv_conv_sum_r _ _ _ _ H)).
-  unfold is_low_sort ; rewrite H2 ; auto.
-  unfold is_low_sort ; rewrite H0 ; auto.
-
-  simpl in H0.
-  apply (IHA2 B2 (inv_conv_sum_r _ _ _ _ H)).
-  unfold is_low_sort ; rewrite H2 ; auto.
-  unfold is_low_sort ; rewrite H0 ; auto.
-
-  induction B ; simpl ; intros ; 
-  try unfold is_low_sort in H1 ;   
-  intuition ; try discriminate ; auto with coc core datatypes.
-
-  elim conv_sort_sum with s A1 A2 ; auto with coc core.
-  elim conv_sort_sum with s A1 A2 ; auto with coc core.
-
-  elim conv_prod_sum with B1 B2 A1 A2; auto with coc core.
-  elim conv_prod_sum with B1 B2 A1 A2; auto with coc core.
-
-  simpl in H0.
-  apply (IHA2 B2 (inv_conv_sum_r _ _ _ _ H)).
-  unfold is_low_sort ; rewrite H2 ; auto.
-  unfold is_low_sort ; rewrite H0 ; auto.
-
-  simpl in H0.
-  apply (IHA2 B2 (inv_conv_sum_r _ _ _ _ H)).
-  unfold is_low_sort ; rewrite H2 ; auto.
-  unfold is_low_sort ; rewrite H0 ; auto.
-Qed.
-
-Lemma conv_is_low_dom_full : forall A B, conv A B ->
-  is_low_sort (type_dom A) -> 
-  is_low_sort (type_dom B) -> type_dom A = type_dom B.
-Proof.
-  induction A ; simpl ; intros ; 
-  try unfold is_low_sort in H0 ;   
-  intuition ; try discriminate ; auto with coc core datatypes.
-  
-  rewrite (conv_is_low_dom H H1).
-  simpl ; auto.
-
-  rewrite (conv_is_low_dom H H1).
-  simpl ; auto.
-  
-  induction B ; simpl ; intros ; 
-  try unfold is_low_sort in H1 ;   
-  intuition ; try discriminate ; auto with coc core datatypes.
-
-  elim conv_sort_sum with s A1 A2 ; auto with coc core.
-  elim conv_sort_sum with s A1 A2 ; auto with coc core.
-
-  simpl in H0.
-  apply (conv_is_low_range_full (inv_conv_sum_l _ _ _ _ H)).
-  rewrite H2 ; unfold is_low_sort ; auto.
-  rewrite H0 ; unfold is_low_sort ; auto.
-
-  simpl in H0.
-  apply (conv_is_low_range_full (inv_conv_sum_l _ _ _ _ H)).
-  unfold is_low_sort ; rewrite H2 ; try rewrite H0 ; auto.
-  unfold is_low_sort ; try rewrite H0 ; auto.
-
-  induction B ; simpl ; intros ; 
-  try unfold is_low_sort in H1 ;   
-  intuition ; try discriminate ; auto with coc core datatypes.
-
-  elim conv_sort_sum with s A1 A2 ; auto with coc core.
-  elim conv_sort_sum with s A1 A2 ; auto with coc core.
-
-  simpl in H0.
-  apply (conv_is_low_range_full (inv_conv_sum_l _ _ _ _ H)).
-  rewrite H2 ; unfold is_low_sort ; auto.
-  rewrite H0 ; unfold is_low_sort ; auto.
-
-  simpl in H0.
-  apply (conv_is_low_range_full (inv_conv_sum_l _ _ _ _ H)).
-  unfold is_low_sort ; rewrite H2 ; try rewrite H0 ; auto.
-  unfold is_low_sort ; try rewrite H0 ; auto.
 Qed.
 
 
@@ -316,11 +92,6 @@ Proof.
   induction 1 ; simpl ; intros ; try discriminate ; auto with coc.
   
   apply IHtyp2 with s ; auto.
-  pose (IHtyp2 s H2) ; auto.
-  inversion e0.
-  rewrite H4 in H1.
-  destruct H1 ; intuition ; try discriminate.
-  rewrite H6 ; auto.
   
   rewrite (IHtyp1 _ H3) in H1.
   elim typ_not_kind2 with e (Srt s) ; auto.
@@ -337,7 +108,7 @@ Proof.
   unfold not ; intros ; discriminate.
 Qed.
 
-
+(*
 Lemma term_type_dom_kinded : forall e t T, e |- t : T ->
   forall s, type_dom t = Srt s -> T = Srt kind. 
 Proof.
@@ -347,21 +118,11 @@ Proof.
   inversion e0.
   rewrite H4 in H1.
   destruct H1 ; intuition ; try discriminate.
-  rewrite H6 ; auto.
   
   rewrite (IHtyp1 _ H3) in H1.
   elim typ_not_kind2 with e (Srt s) ; auto.
 Qed.
-
-Lemma is_prop_is_low_sort : forall s, is_prop s -> is_low_sort (Srt s).
-Proof.
-  intros.
-  destruct H ; unfold is_low_sort ; intuition.
-  rewrite H ; auto.
-  rewrite H ; auto.
-Qed.
-
-
+*)
 Lemma conv_sum_ref : forall U V n, ~ conv (Sum U V) (Ref n).
 Admitted.
 Lemma conv_prod_ref : forall U V n, ~ conv (Prod U V) (Ref n).
@@ -440,316 +201,39 @@ Qed.
 *)
 
 Lemma conv_dom : 
-  forall e A Ts, e |- A : Ts -> 
-  forall B s s', Ts = Srt s -> 
-  forall s'', e |- B : Srt s'' -> conv A B -> 
-  (s = s'') /\
-  (type_dom A = Srt s' -> type_dom B = Srt s')
-  /\ (type_range A = Srt s' -> type_range B = Srt s')
-  .
+  forall A B, conv A B -> 
+  forall s', 
+  is_low_full A -> is_low_full B ->
+  (type_range A = Srt s' -> type_range B = Srt s').
 Proof.
-  induction 1 ; simpl ; intros ; try discriminate.
+  induction A ; simpl ; intros ; try discriminate ; try contradiction.
   
-  split.
-  pose (sort_conv_eq).
-
-  inversion H0.
-  rewrite <- H5 in H1.
-  pose (sort_conv_eq H1 (sym_conv _ _ H2)).
-  rewrite e0.
-  simpl.
+  induction B ; simpl ; intros ; try discriminate ; try contradiction.
+  pose (conv_sort _ _ H).
+  rewrite <- e.
   auto.
 
-  inversion H0.
-  rewrite <- H4 in H1.
-  pose (sort_conv_eq H1 (sym_conv _ _ H2)).
-  rewrite e0.
-  simpl.
-  auto.
+  elim conv_sort_prod with s B1 B2 ; auto with coc.
 
-  split ; intros ; discriminate.
+  induction B ; simpl ; intros ; try discriminate ; try contradiction.
 
-  split ; intros ; discriminate.
+  elim conv_sort_prod with s A1 A2 ; auto with coc.
 
-  split ; intros ; try discriminate.
-
-  induction B ; simpl ; intros ; try discriminate.
-  
-  elim conv_sort_prod with s0 T U ; auto with coc.
-  elim conv_prod_ref with T U n ; auto with coc.
-  elim conv_prod_abs with T U B1 B2 ; auto with coc.
-
-  pose (term_type_range_kinded H0 H4).
-  rewrite H1 in e0.
-  inversion e0.
-  rewrite H6 in H2.
-  pose (gen_sorting_app H2).
-  destruct i ; discriminate.
-  elim conv_prod_pair with T U B1 B2 B3 ; auto.
-
-  destruct (IHtyp2 B2 s s') ; auto with coc.
-  destruct (generation_prod2 H2).
-  apply typ_conv_env with (B1 :: e) ; auto with coc core.
-  destruct H5.
-
-  inversion H1.
-  assert (e |- Prod T U : Srt s).
-  rewrite <- H8.
-  apply type_prod with s1 ; auto.
-  pose (inv_conv_prod_sort_l H7 H2 H3).
-  destruct s0.
-  intuition.
-  pose (inv_conv_prod_l _ _ _ _ H3).
-  apply coerce_env_hd with x0.
-  apply coerce_conv with T T ; auto with coc.
-
-  apply wf_var with s1 ; auto with coc.
-  apply (inv_conv_prod_r _ _ _ _ H3).
-
-  elim conv_prod_sum with T U B1 B2 ; auto with coc.
-
-  elim conv_prod_subset with T U B1 B2 ; auto with coc.
-
-  pose (term_type_range_kinded H0 H4).
-  rewrite H1 in e0.
-  inversion e0.
-  rewrite H6 in H2.
-  pose (gen_sorting_pi1 H2).
-  destruct i ; discriminate.
-
-  pose (term_type_range_kinded H0 H4).
-  rewrite H1 in e0.
-  inversion e0.
-  rewrite H6 in H2.
-  pose (gen_sorting_pi2 H2).
-  destruct i ; discriminate.
-
-  elim (not_t_let_in H2) with B1 B2 ; auto with coc.
-
-  induction B ; simpl ; intros ; try discriminate.
-  
-  elim conv_sort_sum with s0 T U ; auto with coc.
-  elim conv_sum_ref with T U n ; auto with coc.
-  elim conv_sum_abs with T U B1 B2 ; auto with coc.
-
-  split ; intros.
-  pose (term_type_range_kinded H H5).
-  inversion e0.
-  rewrite H7 in H1.
-  induction H1 ; intuition ; try discriminate.
-  rewrite H9 in H2.
-  inversion H2.
-  rewrite <- H10 in H3.
-  pose (gen_sorting_app H3).
-  destruct i ; discriminate.
-
-  pose (term_type_range_kinded H0 H5).
-  inversion e0.
-  rewrite H7 in H1.
-  induction H1 ; intuition ; try discriminate.
-  rewrite H9 in H2.
-  inversion H2.
-  rewrite <- H10 in H3.
-  pose (gen_sorting_app H3).
-  destruct i ; discriminate.
-
-  elim conv_sum_pair with T U B1 B2 B3 ; auto.
-
-  elim conv_prod_sum with B1 B2 T U ; auto with coc.
-
-  assert (e |- Sum T U : Srt s3).
-  apply type_sum with s1 s2 ; auto.
-  inversion H2.
-  rewrite H7 in H5.
-  rewrite H7 in H1.
-  destruct (inv_conv_sum_sort H5 H3 H4).
-  destruct H6.
-  destruct H6.
-  destruct H8.
-  destruct H9.
-  destruct H10.
-      
-  pose (inv_conv_sum_l _ _ _ _ H4).
-  pose (inv_conv_sum_r _ _ _ _ H4).
-
-  split ; intros.
-  induction H1 ; induction H11 ; intuition ; try rewrite H12 ; try rewrite H1 ; try rewrite H11 ; try discriminate ;
-  try (rewrite H15 in H17 ; discriminate) ; auto.
-  rewrite H13 in H.
-  pose (term_type_range_kinded H H12) ; discriminate.
-
-  rewrite H13 in H.
-  pose (term_type_range_kinded H H12) ; discriminate.
-  rewrite H13 in H.
-  pose (term_type_range_kinded H H12) ; discriminate.
-
-  pose (term_type_range_kinded H H5) ; discriminate.
-
-  destruct (IHtyp1 B1 x s') ; auto with coc. 
-  induction H1 ; induction H11 ; intuition ; try rewrite H12 ; try rewrite H1 ; try rewrite H11 ; try discriminate ;
-  try (rewrite H14 in H16 ; discriminate) ; auto.
-
-  
-  
-
-
-
-  pose (IHtyp2 B2 s s') ; auto with coc.
-  destruct (generation_prod2 H2).
-  apply typ_conv_env with (B1 :: e) ; auto with coc core.
-  destruct H5.
-
-  inversion H1.
-  assert (e |- Prod T U : Srt s).
-  rewrite <- H8.
-  apply type_prod with s1 ; auto.
-  pose (inv_conv_prod_sort_l H7 H2 H3).
-  destruct s0.
-  intuition.
-  pose (inv_conv_prod_l _ _ _ _ H3).
-  apply coerce_env_hd with x0.
-  apply coerce_conv with T T ; auto with coc.
-
-  apply wf_var with s1 ; auto with coc.
-  apply (inv_conv_prod_r _ _ _ _ H3).
-
-
-  elim conv_subset_sum with B1 B2 T U ; auto with coc.
-
-  pose (term_type_range_kinded H0 H4).
-  rewrite H1 in e0.
-  inversion e0.
-  rewrite H6 in H2.
-  pose (gen_sorting_pi1 H2).
-  destruct i ; discriminate.
-
-  pose (term_type_range_kinded H0 H4).
-  rewrite H1 in e0.
-  inversion e0.
-  rewrite H6 in H2.
-  pose (gen_sorting_pi2 H2).
-  destruct i ; discriminate.
-
-  elim (not_t_let_in H2) with B1 B2 ; auto with coc.
-
-
-
-  Focus 2.
-  split ; intros ; discriminate.
-  Focus 2.
-  split ; intros ; discriminate.
-  Focus 2.
-  split ; intros ; discriminate.
-  Focus 2.
-  rewrite H3 in H2.
-  pose (coerce_propset_r H2).
-  apply (IHtyp1 B s0 s' e0 H4 H5).
-
-
-
-  destruct (IHtyp2 B2 s s') ; auto with coc.
-  destruct (generation_prod2 H2).
-  apply typ_conv_env with (B1 :: e) ; auto with coc core.
-  destruct H5.
-
-  inversion H1.
-  assert (e |- Prod T U : Srt s).
-  rewrite <- H8.
-  apply type_prod with s1 ; auto.
-  pose (inv_conv_prod_sort_l H7 H2 H3).
-  destruct s0.
-  intuition.
-  pose (inv_conv_prod_l _ _ _ _ H3).
-  apply coerce_env_hd with x0.
-  apply coerce_conv with T T ; auto with coc.
-
-  apply wf_var with s1 ; auto with coc.
-  apply (inv_conv_prod_r _ _ _ _ H3).
-
-
-  pose (IHtyp1 
-  apply coerce_conv with B1 B1 ; auto with coc.
-
-Focus 2.
-  apply IHtyp1 with s0 ; auto.
-  rewrite H3 in H2.
-  apply (coerce_propset_r H2).
-
-  pose (term_type_range_kinded H H4).
-  
-  induction H1 ; intuition.
-  rewrite H6 in e0 ; discriminate.
-
-  induction B ; simpl ; intros ; try discriminate.
-
-  elim conv_sort_sum with s0 T U ; auto with coc.
-
-  elim conv_sum_ref with T U n ; auto.
-
-  elim (sorting_lambda H3).
-
-  inversion H2.
-  rewrite <- H9 in H3.
-  rewrite H8 in H3.
-  pose (gen_sorting_app H3).
-  destruct i ; discriminate.
-
-  elim conv_sum_pair with T U B1 B2 B3 ; auto.
-
-  elim conv_prod_sum with B1 B2 T U ; auto with coc.
-  inversion H2.
-  rewrite <- H9 in H3.
-  pose (generation_sum2 H3).
-  destruct e1 ; intuition.
-  destruct H11.
-  intuition.
-  induction H12 ; intuition ; try discriminate.
-  rewrite H8 in H14 ; discriminate.
-  rewrite H7 in H10.
-  rewrite H1 in IHtyp1.
-  pose (IHtyp1 kind (refl_equal (Srt kind)) B1 H10).
-
-  intros.
-
-  
-
-
-(*
-Lemma type_range_conv : forall e T U s, conv T U -> e |- T : Srt kind -> e |- U : Srt kind ->
-  forall s0, type_range T = Srt s0 -> type_range U = Srt s0.
-Proof.
-  intros.
-  *)
-
+  pose (inv_conv_prod_r _ _ _ _ H).
+  simpl in H1.
+  apply (IHA2 _ c s' H0 H1).
+  assumption.
+Qed.
 
 Lemma type_range_sub : forall e T U s, e |- T >> U : s ->
-  forall s0, (type_range U = Srt s0 -> type_range T = Srt s0) /\
-  (type_dom U = Srt s0 -> type_dom T = Srt s0).
+  forall s0, (type_range U = Srt s0 -> type_range T = Srt s0).
 Proof.
   induction 1 ; simpl ; intros ; try discriminate ; auto with coc.
 
-  destruct (IHcoerce1 s). 
-  destruct (IHcoerce2 s0).
-  split ; intros ; auto.
-  discriminate.
-
-  destruct (IHcoerce1 s0). 
-  destruct (IHcoerce2 s0).
-  split ; intros ; auto.
-
   pose (coerce_sort_r H).
-  destruct (IHcoerce s0). 
-  split ; intros ; auto.
-
-  pose (term_type_range_kinded t H3).
+  
+  pose (term_type_range_kinded t H1).
   discriminate.
-
-  pose (coerce_sort_l H).
-  pose (term_type_dom_kinded t H3).
-  discriminate.
-
-  split ; intros ; discriminate.
-  split ; intros.
 
   pose (term_type_range_kinded H2 H6).
   inversion e0.
@@ -761,218 +245,11 @@ Proof.
   pose (sort_of_kinded H0).
   pose (sort_of_kinded H1).
   pose (sort_of_kinded H7).
-  destruct (is_low_type_range H7 i2).
-  pose (H9 s0) ; contradiction.
-  do 2 destruct H9.
-  
-  pose (is_prop_is_low_sort H10).
-  rewrite <- H9 in i3.
-
-  destruct (is_low_type_range H1 i1).
-  
-  
-Focus 2.
-  pose (H9 s0) ; contradiction.
-  do 2 destruct H9.
-  
-  pose (is_prop_is_low_sort H10).
-  rewrite <- H9 in i3.
-
-  assert(is_low_sort (type_range D)).
-  rewrite H9 ; unfold is_low_sort ; destruct H10 ; simpl ; auto.
-  rewrite H10 ; auto.
-  rewrite H10 ; auto.
-
-
-  pose (conv_is_low_range_full H3 H11 i0).
-  
-  pose (is_low_type_range H0).
-  pose (is_low_type_range H0).
-
-
-  pose (type_kind_range H1).
-  pose (type_kind_range H7).
-  
-  pose (conv_is_low_range_full H5 i1 i2).
-  rewrite H6 in e2.
-  pose (IHcoerce _ e2).
-  rewrite <- e3.
-  assumption.
+  pose (@conv_dom _ _ (sym_conv _ _ H5) s0 i2 i1).
+  pose (e1 H6).
+  pose (IHcoerce s0 e2).
+  apply (@conv_dom _ _  (sym_conv _ _ H3) s0 i0 i) ; auto.
 Qed.
-
-
-
-
-
-Lemma type_dom_sub : forall e T U s, e |- T >> U : s ->
-  forall s0, type_dom U = Srt s0 -> type_dom T = Srt s0.
-Proof.
-  induction 1 ; simpl ; intros ; try discriminate ; auto with coc.
-
-  apply type_range_sub with e A' s ; auto with coc.
-
-  pose (coerce_sort_r H).
-  pose (term_type_dom_kinded t H1).
-  discriminate.
-  
-  induction D ; simpl in H6 ; try discriminate.
-
-  destruct (typ_sort H2).
-  inversion H8.
-  rewrite H10 in H1.
-  pose (type_kind_range H1).
-  pose (conv_is_low_range (sym_conv _ _ H5) i).
-  rewrite e0 in IHcoerce.
-  inversion H6.
-  assert (type_dom B = Srt s0).
-  apply IHcoerce.
-  rewrite H11 ; simpl ; auto.
-
-  pose (sort_conv_eq H1 H5).
-  rewrite e1 in H4.
-  pose (coerce_propset_r H4).
-  rewrite e2 in H3.
-  rewrite H10 in H.
-  pose (sort_conv_eq H H3).
-  rewrite e3 ; simpl ; auto.
-
-  pose (generation_sum2 H2).
-  destruct e0.
-  intuition.
-  pose (term_type_range_kinded H8 H6).
-  inversion e0.
-
-  pose (term_type_dom_kinded H2 H6).
-  inversion e1.
-
-  
-  rewrite H8 in H.
-  rewrite H8 in H0.
-  rewrite H8 in H1.
-  rewrite H8 in H2.
-  pose (type_kind_dom H).
-  pose (type_kind_dom H0).
-  pose (type_kind_dom H1).
-  pose (type_kind_dom H7 H6).
-  
-
-
-  pose (conv_is_low_dom_full H3).
-  pose (conv_is_low_range_full H5 i1 i2).
-  rewrite H6 in e2.
-  pose (IHcoerce _ e2).
-  rewrite <- e3.
-  assumption.
-
-
-
-  unfold sum_sort in H10.
-  intuition.
-  rewrite H10 in H6.
-  simpl in H9 ; inversion H9.
-  
-  
-
-  Focus 2.
-  
-
-rewrite H10 in H.
-  pose (type_kind_range H).
-  pose(conv_is_low_range).
-  induction i.
-  pose (term_type_range_
-
-  pose (conv_is_low_range).
- 
-  pose (term_type_dom_kinded H2 H6).
-  inversion e0.
-  rewrite H8 in H.
-  rewrite H8 in H0.
-  rewrite H8 in H1.
-  clear e0.
-  rewrite H8 in H2.
-  pose (type_kind_dom H2 H6).
-
-  pose (conv_is_low_dom_full).
-  
-  pose (type_kind_dom H).
-  pose (type_kind_range H0).
-  pose (type_kind_range H1).
-  pose (conv_is_low_dom_full H3 i i0).
-  pose (conv_is_low_dom_full H5 i1 i2).
-  rewrite H6 in e2.
-  pose (IHcoerce _ e2).
-  rewrite <- e3.
-  assumption.
-
-  induction B ; try discriminate.
-  simpl in H2.
-
-  inversion H2.
-  induction (typ_sort _ _ _ H0).
-  inversion H5.
-  rewrite H7 in H.
-  pose (kind_is_prod H (refl_equal (Srt kind))).
-  rewrite (conv_is_low_range (sym_conv _ _ H1) i).
-  simpl ; assumption.
-
-  rewrite <- H2.
-  simpl in H2.
-  destruct (generation_prod2 H0).
-  induction H3.
-  pose (term_type_range_kinded H3 H2).
-  inversion e0.
-  rewrite H6 in H3.
-
-  simpl.
-  rewrite H2.
-  
-  pose (conv_is_low_dom_full).
-
-Focus 4.
-  pose (coerce_sym _ _ _ _ H).
-  exact (type_range_sub c H5).
-
-Focus 4.
-  exact (type_range_sub H H5).
-
-Focus 4.
-  pose (IHcoerce _ H1).
-  pose (coerce_sort_l _ _ _ _ H).
-  pose (term_type_range_kinded t e0).
-  
-
-  induction A ; try discriminate.
-  
-  elim conv_sort_prod with s1 B1 B2 ; auto.
-  elim conv_ref_prod with n B1 B2 ; auto.
-  elim conv_abs_prod with A1 A2 B1 B2 ; auto.
-  simpl.
-  
-
-  apply IHB1.
-
-
-  apply (conv_is_low_dom_full H1).
-  
-
-apply kind_is_prod with e (Srt s) ; auto.
-  apply kind_is_prod with e (Srt s) ; auto.
-
-  rewrite <- H2.
-  pose (term_type_range_kinded H0 H2).
-  inversion e0.
-  rewrite H4 in H0.
-  
-  apply (conv_is_low_range_full H1).
-  apply kind_is_prod with e (Srt s) ; auto.
-  apply kind_is_prod with e (Srt s) ; auto.
-
-  pose (coerce_sort_r _ _ _ _ H).
-  pose (term_type_range_kinded t H1).
-  discriminate.
-Qed.
-*)
 
 Lemma var_sort_range_item_aux : forall e t T, e |- t : T ->
   forall n, t = Ref n -> 
@@ -1000,13 +277,6 @@ Proof.
   intuition ; auto.
   rewrite <- H5 ; assumption.
   
-  inversion H1.
-  exists (Sum T1 T2).
-  intuition ; auto.
-  rewrite <- H5 ; assumption.
-
-
-
   exact (IHtyp1 n H3 s0 (type_range_sub H2 H4)).
 Qed. 
 
@@ -1136,134 +406,122 @@ Qed.
 
 *)
 
-
 Lemma sort_of_pair_range_aux : forall e t Ts, e |- t : Ts ->
   forall T u v, t = Pair T u v ->
-  forall s, type_range Ts = Srt s ->
-  exists U, exists V, exists s1, exists s2,
-  T = Sum U V /\
-  e |- u : U /\ e |- U : Srt s1 /\ U :: e |- V : Srt s2 /\
-  e |- v : subst u V /\ e |- Sum U V : Srt s2 /\ 
-  type_range V = (Srt s).
+  forall s, type_range Ts <> Srt s.
 Proof.
   induction 1 ; simpl ; intros ;
   auto with coc core arith datatypes ; try discriminate.
 
-  exists U ; exists V ; exists s1 ; exists s2.
-  inversion H4.
-  rewrite <- H9 ; rewrite <- H8.
-  intuition.
-  apply type_sum with s1 ; auto.
-
-  apply IHtyp1 ; auto.
-  apply (type_range_sub H2 H4).
+  unfold not ; intros.
+  pose (type_range_sub H2 H4).
+  pose (IHtyp1 _ _ _ H3 s0).
+  contradiction.
 Qed.
 
 Lemma sort_of_pair_range : forall e T u v Ts, e |- Pair T u v : Ts ->
-  forall s, type_range Ts = Srt s ->
-  exists U, exists V, exists s1, exists s2,
-  T = Sum U V /\
-  e |- u : U /\ e |- U : Srt s1 /\ U :: e |- V : Srt s2 /\
-  e |- v : subst u V /\ e |- Sum U V : Srt s2 /\ 
-  type_range V = (Srt s).
+  forall s, type_range Ts <> Srt s.
 Proof.
   intros. 
-  apply sort_of_pair_range_aux with (Pair T u v) Ts  ; auto ; auto.
+  apply (@sort_of_pair_range_aux e (Pair T u v) Ts H T u v) ; auto ; auto.
+Qed.
+
+Lemma sum_sort_prop : forall s s' s'', sum_sort s s' s'' -> 
+  is_prop s /\ s = s' /\ s' = s''.
+Proof.
+  induction 1.
+  destruct H.
+  destruct H0.
+  rewrite H ; rewrite H0 ; rewrite H1.
+  unfold is_prop ; intuition.
+  destruct H.
+  destruct H0.
+  rewrite H ; rewrite H0 ; rewrite H1.
+  unfold is_prop ; intuition.
+Qed.
+
+Lemma sort_of_sum_aux : forall e T Ts, e |- T : Ts -> 
+  forall U V, T = Sum U V -> 
+  (forall s, type_range U <> Srt s) /\ 
+  (forall s, type_range V <> Srt s).
+Proof.
+  induction 1 ; simpl ; intros ;
+  auto with coc core arith datatypes ; try discriminate.
+  
+  pose (sum_sort_prop H1).
+  destruct a.
+  destruct H4.
+  rewrite <- H4 in H0.
+  pose (sort_of_propset H H3).
+  pose (sort_of_propset H0 H3).
+  pose (no_sort_type_range _ n).
+  pose (no_sort_type_range _ n0).
+  inversion H2.
+  rewrite <- H7.
+  rewrite <- H8.
+  intuition.
+Qed.
+
+Lemma sort_of_sum : forall e U V T, e |- Sum U V : T -> 
+  (forall s, type_range U <> Srt s) /\ 
+  (forall s, type_range V <> Srt s).
+Proof.
+  intros ; apply sort_of_sum_aux with e (Sum U V) T ; auto ; auto.
 Qed.
 
 Lemma sort_of_pi1_range_aux : forall e t Ts, e |- t : Ts ->
   forall u, t = Pi1 u ->
-  forall s, type_range Ts = Srt s ->
-  exists U, exists V, exists s2, 
-  e |- u : Sum U V /\ type_range U = (Srt s)
-  /\ sum_sort U V s s2.
+  forall s, type_range Ts <> Srt s.
 Proof.
   induction 1 ; simpl ; intros ;
   auto with coc core arith datatypes ; try discriminate.
-  
+
   induction (type_sorted H) ; try discriminate.
-  induction H2.
-  induction (generation_sum2 H2).
-
-  exists U ; exists V.
-  inversion H0.
-  rewrite <- H5.
-  exists x.
-  intuition.
-  pose (term_type_range_kinded H4 H1).
-  inversion e0.
-  rewrite H8 in H7.
-  unfold sum_sort in H7.
-  destruct H7.
-  induction H6 ; try discriminate.
-  unfold sum_sort.
-  intuition.
+  induction H1.
+  induction (sort_of_sum H1).
+  apply H2 ; auto.
   
-  destruct H6.
-  discriminate.
-
-  apply IHtyp1 ; auto.
-  apply (type_range_sub H2 H4).
+  red ; intros.
+  pose (type_range_sub H2 H4).
+  apply (IHtyp1 _ H3 s0 e0).
 Qed.
 
 Lemma sort_of_pi1_range :  forall e t Ts, e |- Pi1 t : Ts ->
-  forall s, type_range Ts = Srt s ->
-  exists U, exists V, exists s2, e |- t : Sum U V /\ type_range U = (Srt s)
-  /\ sum_sort U V s s2.
+  forall s, type_range Ts <> Srt s.
 Proof.
   intros. 
-  apply sort_of_pi1_range_aux with (Pi1 t) Ts  ; auto ; auto.
+  apply (@sort_of_pi1_range_aux _ _ _  H t) ; auto ; auto.
 Qed.
 
 Lemma sort_of_pi2_range_aux : forall e t Ts, e |- t : Ts ->
   forall u, t = Pi2 u ->
-  forall s, type_range Ts = Srt s ->
-  exists U, exists V, exists s1, 
-	e |- u : Sum U V /\ type_range (subst (Pi1 u) V) = (Srt s)
-	/\ sum_sort U V s1 s.
+  forall s, type_range Ts <> Srt s.
 Proof.
   induction 1 ; simpl ; intros ;
   auto with coc core arith datatypes ; try discriminate.
 
   induction (type_sorted H) ; try discriminate.
-  induction H2.
-  induction (generation_sum2 H2).
-
-  exists U ; exists V.
-  inversion H0.
-  rewrite <- H5.
-  exists x0.
-  intuition.
-
-  unfold sum_sort in H7 |- *.
-  destruct H7.
-  left ; intuition.
-  right.
-  split ; intuition.
+  induction H1.
+  induction (sort_of_sum H1).
+  red ; intros.
   
-  induction (type_range_subst _ _ _ H1).
-  simpl in H6.
-  discriminate.
+  induction (type_range_subst _ _ _ H4).
+  simpl in H5 ; discriminate.
+  pose (H3 s);contradiction.
 
-  pose (term_type_range_kinded H3 H6).
-  inversion e0.
-  rewrite H10 in H8.
-  discriminate.
-  
-  apply IHtyp1 ; auto.
-  apply (type_range_sub H2 H4).
+  red ; intros.
+  pose (type_range_sub H2 H4).
+  apply (IHtyp1 u H3 s0 e0) ; auto.
 Qed.
 
 Lemma sort_of_pi2_range :  forall e t Ts, e |- Pi2 t : Ts ->
-  forall s, type_range Ts = Srt s ->
-  exists U, exists V, exists s1, e |- t : Sum U V /\ type_range (subst (Pi1 t) V) = (Srt s)
-  /\ sum_sort U V s1 s.
+  forall s, type_range Ts <> Srt s.
 Proof.
   intros. 
-  apply sort_of_pi2_range_aux with (Pi2 t) Ts  ; auto ; auto.
+  apply sort_of_pi2_range_aux with e (Pi2 t) t  ; auto ; auto.
 Qed.
 
-Lemma sort_of_letin_range_aux : forall e t Ts, e |- t : Ts ->
+(*Lemma sort_of_letin_range_aux : forall e t Ts, e |- t : Ts ->
   forall u v, t = Let_in u v ->
   forall s, type_range Ts = Srt s ->
   exists U, exists V, 
@@ -1291,7 +549,7 @@ Proof.
   intros. 
   apply sort_of_letin_range_aux with (Let_in u v) Ts  ; auto ; auto.
 Qed.
-
+*)
 Lemma type_range_subst2 : forall t u n s, type_range t = Srt s -> 
   type_range (subst_rec u t n) = Srt s.
 Proof.
