proof/Russell/UnicityOfSortingRange.v
@@ -22,22 +22,19 @@ Set Implicit Arguments.
 
 Lemma unique_range_sort : forall t e T T', e |- t : T -> e |- t : T' -> 
 forall s1 s2, 
-(type_range T = Srt s1 -> type_range T' = Srt s2 -> s1 = s2) /\
-(type_dom T = Srt s1 -> type_dom T' = Srt s2 -> s1 = s2).
+(type_range T = Srt s1 -> type_range T' = Srt s2 -> s1 = s2).
 Proof.
   induction t ; simpl ; intros ; 
   auto with coc core arith datatypes ; try discriminate.
 
   destruct (typ_sort H).
   destruct (typ_sort H0).
-  rewrite H4.
-  rewrite H2.
-  simpl.
-  split ; intros ; intuition;
-  inversion H5 ; inversion H6 ;  auto.
+  rewrite H4 in H1.
+  rewrite H6 in H2.
+  simpl in H1, H2.
+  inversion H1 ; inversion H2 ; auto.
 
   (* Var *)
-  exact (unique_var_range_sort H H1 H0 H2).
   exact (unique_var_range_sort H H1 H0 H2).
     
   (* Abs *)  
@@ -58,7 +55,7 @@ Proof.
 
   pose (term_type_range_kinded H4 H8).
   rewrite e0 in H3.
-  pose (type_no_kind_prod_type2 H3).
+  pose (type_no_kind_prod_type H3).
   simpl in t.
   intuition.
 
@@ -69,25 +66,18 @@ Proof.
 
   pose (term_type_range_kinded H4 H5).
   rewrite e0 in H3.
-  pose (type_no_kind_prod_type2 H3).
+  pose (type_no_kind_prod_type H3).
   simpl in t.
   intuition.
 
   pose (term_type_range_kinded H4 H5).
   rewrite e0 in H3.
-  pose (type_no_kind_prod_type2 H3).
+  pose (type_no_kind_prod_type H3).
   simpl in t.
   intuition.
 
   (* Pair *)
   induction (sort_of_pair_range H H1).
-  do 3 destruct H3 ; intuition.
-  induction (sort_of_pair_range H0 H2).
-  do 3 destruct H9 ; intuition.
-
-  apply (IHt3 _ _ _ H7 H14) ; simpl ; auto.
-  unfold subst ; apply type_range_subst2 ; auto.
-  unfold subst ; apply type_range_subst2 ; auto.
   
   (* Prod *)
   induction (generation_prod H).
@@ -106,12 +96,8 @@ Proof.
   rewrite H3 in H.
   rewrite H4 in H0.
   induction (generation_sum2 H).
-  destruct H5.
-  destruct H6.
   induction (generation_sum2 H0).
-  destruct H8.
-  destruct H9.
-  apply (IHt2 _ _ _ H6 H9).
+  apply (IHt2 _ _ _ H6 H8).
   rewrite <- H3 ; auto.
   rewrite <- H4 ; auto.
 
@@ -126,67 +112,11 @@ Proof.
 
   (* Pi1 *)
   induction (sort_of_pi1_range H H1).
-  do 2 destruct H3 ; intuition.
-  induction (sort_of_pi1_range H0 H2).
-  do 2 destruct H5 ; intuition.
-  
-  unfold sum_sort in H6.
-  destruct H6.
-
-  unfold sum_sort in H9.
-  destruct H9.
-
-  intuition.
-  
-  apply (IHt _ _ _ H4 H7) ; simpl ; auto.
-  rewrite H10.
-  rewrite <- H3.
-  rewrite H9 ; auto.
-
-  rewrite H11.
-  rewrite H6 in H5.
-  assumption.
-
-  destruct H8.
-  destruct H6.
-  rewrite H8.
-  rewrite H6 in H3.
-  simpl in H3.
-  inversion H3 ; auto.
-
-  unfold sum_sort in H9.
-  destruct H9.
-  
-  intuition.
-
-  rewrite H9.
-  rewrite H6 in H5.
-  simpl in H5.
-  inversion H5 ; auto.
-
-  intuition.
-  rewrite H6 ; rewrite H9 ; auto.
 
   (* Pi2 *)
   induction (sort_of_pi2_range H H1).
-  do 2 destruct H3 ; intuition.
-  induction (sort_of_pi2_range H0 H2).
-  do 2 destruct H5 ; intuition.
-  
-  apply (IHt _ _ _ H4 H7) ; simpl.
-  unfold subst in H3 ; induction (type_range_subst _ _ _ H3).
-  simpl in H8 ; discriminate.
-  assumption.
 
-  unfold subst in H5 ; induction (type_range_subst _ _ _ H5).
-  simpl in H8 ; discriminate.
-  assumption.
-
-  induction (sort_of_letin_range H H1).
-  destruct H3 ; intuition.
-  induction (sort_of_letin_range H0 H2).
-  destruct H5 ; intuition.
-
+  (* Let_in *)
   elim (@not_t_let_in _ _ _ H t1 t2).
   auto.
 Qed.
